StrataTest/DL/Lambda/Lambda.lean
@@ -37,7 +37,9 @@ New Function:func Int.Add :  () → int;
 
 /--
 info: Annotated expression:
-(((~Int.Le : (arrow int (arrow int bool))) (((~Int.Div : (arrow int (arrow int int))) #300) (((~Int.Add : (arrow int (arrow int int))) #2) #1))) #100)
+((~Int.Le : (arrow int (arrow int bool)))
+ ((~Int.Div : (arrow int (arrow int int))) #300 ((~Int.Add : (arrow int (arrow int int))) #2 #1))
+ #100)
 
 ---
 info: #true
@@ -48,10 +50,10 @@ info: #true
 
 /--
 info: Annotated expression:
-((~Int.Div : (arrow int (arrow int int))) (((~Int.Add : (arrow int (arrow int int))) #2) #1))
+((~Int.Div : (arrow int (arrow int int))) ((~Int.Add : (arrow int (arrow int int))) #2 #1))
 
 ---
-info: (λ (((~Int.Div : (arrow int (arrow int int))) #3) %0))
+info: (λ ((~Int.Div : (arrow int (arrow int int))) #3 %0))
 -/
 #guard_msgs in
 #eval format $ typeCheckAndPartialEval TypeFactory.default  (IntBoolFactory : @Factory TestParams)
