StrataTest/Languages/C_Simp/Examples/Coprime.lean
@@ -62,17 +62,29 @@ bool procedure coprime(a:int, b:int)//@pre(a>(0))&&(b>(0));
 
 /--
 info: function coprime {
-  pre: ((~Bool.And ((~Int.Gt a) #0)) ((~Int.Gt b) #0))
+  pre: (~Bool.And (~Int.Gt a #0) (~Int.Gt b #0))
   post: #true
   body:
-init (i : int) := init_i
-i := a
-if ((~Int.Lt b) a) then {i := b}
-else{}
-while (((~Int.Gt i) #1)) (some i) (some #true) {if ((~Bool.And (((~Int.Mod b) i) == #0)) (((~Int.Mod a) i) == #0)) then {return := #false}
- else{}
- i := ((~Int.Sub i) #1)}
-return := #true
+{
+  init (i : int) := init_i
+  i := a
+  if (~Int.Lt b a) {
+    i := b
+  }
+  else {}
+  while
+    (~Int.Gt i #1)
+    (some i)
+    (some #true)
+  {
+    if (~Bool.And ((~Int.Mod b i) == #0) ((~Int.Mod a i) == #0)) {
+      return := #false
+    }
+    else {}
+    i := (~Int.Sub i #1)
+  }
+  return := #true
+}
 }
 Errors: #[]
 -/
@@ -83,33 +95,56 @@ open Strata.C_Simp in
 /--
 info: procedure coprime :  ((a : int) (b : int)) → ((return : bool))
   modifies: []
-  preconditions: (pre, ((~Bool.And ((~Int.Gt a) #0)) ((~Int.Gt b) #0)))
+  preconditions: (pre, (~Bool.And (~Int.Gt a #0) (~Int.Gt b #0)))
   postconditions: (post, #true)
 {
-  init (i : int) := init_i
-  i := a
-  if ((~Int.Lt b) a) then {i := b}
-  else{}
-  if ((~Int.Gt i) #1) then {first_iter_asserts : {assert [entry_invariant] #true
-    assert [assert_measure_pos] ((~Int.Ge i) #0)}
-   arbitrary iter facts : {loop havoc : {havoc return
-     havoc i}
-    arbitrary_iter_assumes : {assume [assume_guard] ((~Int.Gt i) #1)
-     assume [assume_invariant] #true
-     assume [assume_measure_pos] ((~Int.Ge i) #0)}
-    init (special-name-for-old-measure-value : int) := i
-    if ((~Bool.And (((~Int.Mod b) i) == #0)) (((~Int.Mod a) i) == #0)) then {return := #false}
-    else{}
-    i := ((~Int.Sub i) #1)
-    assert [measure_decreases] ((~Int.Lt i) special-name-for-old-measure-value)
-    assert [measure_imp_not_guard] (if ((~Int.Le i) #0) then (~Bool.Not ((~Int.Gt i) #1)) else #true)
-    assert [arbitrary_iter_maintain_invariant] #true}
-   loop havoc : {havoc return
-    havoc i}
-   assume [not_guard] (~Bool.Not ((~Int.Gt i) #1))
-   assume [invariant] #true}
-  else{}
-  return := #true
+  {
+    init (i : int) := init_i
+    i := a
+    if (~Int.Lt b a) {
+      i := b
+    }
+    else {}
+    if (~Int.Gt i #1) {
+      first_iter_asserts :
+      {
+        assert [entry_invariant] #true
+        assert [assert_measure_pos] (~Int.Ge i #0)
+      }
+      arbitrary iter facts :
+      {
+        loop havoc :
+        {
+          havoc return
+          havoc i
+        }
+        arbitrary_iter_assumes :
+        {
+          assume [assume_guard] (~Int.Gt i #1)
+          assume [assume_invariant] #true
+          assume [assume_measure_pos] (~Int.Ge i #0)
+        }
+        init (special-name-for-old-measure-value : int) := i
+        if (~Bool.And ((~Int.Mod b i) == #0) ((~Int.Mod a i) == #0)) {
+          return := #false
+        }
+        else {}
+        i := (~Int.Sub i #1)
+        assert [measure_decreases] (~Int.Lt i special-name-for-old-measure-value)
+        assert [measure_imp_not_guard] (if (~Int.Le i #0) then (~Bool.Not (~Int.Gt i #1)) else #true)
+        assert [arbitrary_iter_maintain_invariant] #true
+      }
+      loop havoc :
+      {
+        havoc return
+        havoc i
+      }
+      assume [not_guard] (~Bool.Not (~Int.Gt i #1))
+      assume [invariant] #true
+    }
+    else {}
+    return := #true
+  }
 }
 -/
 #guard_msgs in
