StrataTest/Languages/C_Simp/Examples/LoopTrivial.lean
@@ -53,14 +53,22 @@ int procedure loopTrivial(n:int)//@pren>=(0);
 
 /--
 info: function loopTrivial {
-  pre: ((~Int.Ge n) #0)
+  pre: (~Int.Ge n #0)
   post: #true
   body:
-init (i : int) := init_i
-i := #0
-while (((~Int.Lt i) n)) (some ((~Int.Sub n) i)) (some ((~Int.Le i) n)) {i := ((~Int.Add i) #1)}
-assert [i_eq_n] (i == n)
-return := i
+{
+  init (i : int) := init_i
+  i := #0
+  while
+    (~Int.Lt i n)
+    (some (~Int.Sub n i))
+    (some (~Int.Le i n))
+  {
+    i := (~Int.Add i #1)
+  }
+  assert [i_eq_n] (i == n)
+  return := i
+}
 }
 Errors: #[]
 -/
@@ -71,28 +79,47 @@ open Strata.C_Simp in
 /--
 info: procedure loopTrivial :  ((n : int)) → ((return : int))
   modifies: []
-  preconditions: (pre, ((~Int.Ge n) #0))
+  preconditions: (pre, (~Int.Ge n #0))
   postconditions: (post, #true)
 {
-  init (i : int) := init_i
-  i := #0
-  if ((~Int.Lt i) n) then {first_iter_asserts : {assert [entry_invariant] ((~Int.Le i) n)
-    assert [assert_measure_pos] ((~Int.Ge ((~Int.Sub n) i)) #0)}
-   arbitrary iter facts : {loop havoc : {havoc i}
-    arbitrary_iter_assumes : {assume [assume_guard] ((~Int.Lt i) n)
-     assume [assume_invariant] ((~Int.Le i) n)
-     assume [assume_measure_pos] ((~Int.Ge ((~Int.Sub n) i)) #0)}
-    init (special-name-for-old-measure-value : int) := ((~Int.Sub n) i)
-    i := ((~Int.Add i) #1)
-    assert [measure_decreases] ((~Int.Lt ((~Int.Sub n) i)) special-name-for-old-measure-value)
-    assert [measure_imp_not_guard] (if ((~Int.Le ((~Int.Sub n) i)) #0) then (~Bool.Not ((~Int.Lt i) n)) else #true)
-    assert [arbitrary_iter_maintain_invariant] ((~Int.Le i) n)}
-   loop havoc : {havoc i}
-   assume [not_guard] (~Bool.Not ((~Int.Lt i) n))
-   assume [invariant] ((~Int.Le i) n)}
-  else{}
-  assert [i_eq_n] (i == n)
-  return := i
+  {
+    init (i : int) := init_i
+    i := #0
+    if (~Int.Lt i n) {
+      first_iter_asserts :
+      {
+        assert [entry_invariant] (~Int.Le i n)
+        assert [assert_measure_pos] (~Int.Ge (~Int.Sub n i) #0)
+      }
+      arbitrary iter facts :
+      {
+        loop havoc :
+        {
+          havoc i
+        }
+        arbitrary_iter_assumes :
+        {
+          assume [assume_guard] (~Int.Lt i n)
+          assume [assume_invariant] (~Int.Le i n)
+          assume [assume_measure_pos] (~Int.Ge (~Int.Sub n i) #0)
+        }
+        init (special-name-for-old-measure-value : int) := (~Int.Sub n i)
+        i := (~Int.Add i #1)
+        assert [measure_decreases] (~Int.Lt (~Int.Sub n i) special-name-for-old-measure-value)
+        assert [measure_imp_not_guard] (if (~Int.Le (~Int.Sub n i) #0) then (~Bool.Not (~Int.Lt i n)) else #true)
+        assert [arbitrary_iter_maintain_invariant] (~Int.Le i n)
+      }
+      loop havoc :
+      {
+        havoc i
+      }
+      assume [not_guard] (~Bool.Not (~Int.Lt i n))
+      assume [invariant] (~Int.Le i n)
+    }
+    else {}
+    assert [i_eq_n] (i == n)
+    return := i
+  }
 }
 -/
 #guard_msgs in
@@ -106,65 +133,125 @@ VCs:
 Label: entry_invariant
 Property: assert
 Assumptions:
-(<label_ite_cond_true: ((~Int.Lt i) n)>, ((~Int.Lt #0) $__n0))
-(pre, ((~Int.Ge $__n0) #0))
+(<label_ite_cond_true: (~Int.Lt i n)>, (~Int.Lt #0 $__n0))
+(pre, (~Int.Ge $__n0 #0))
 
 Proof Obligation:
-((~Int.Le #0) $__n0)
+(~Int.Le #0 $__n0)
 
 Label: assert_measure_pos
 Property: assert
 Assumptions:
-(<label_ite_cond_true: ((~Int.Lt i) n)>, ((~Int.Lt #0) $__n0))
-(pre, ((~Int.Ge $__n0) #0))
+(<label_ite_cond_true: (~Int.Lt i n)>, (~Int.Lt #0 $__n0))
+(pre, (~Int.Ge $__n0 #0))
 
 Proof Obligation:
-((~Int.Ge ((~Int.Sub $__n0) #0)) #0)
+(~Int.Ge (~Int.Sub $__n0 #0) #0)
 
 Label: measure_decreases
 Property: assert
 Assumptions:
-(<label_ite_cond_true: ((~Int.Lt i) n)>, ((~Int.Lt #0) $__n0))
-(assume_guard, ((~Int.Lt $__i2) $__n0)) (assume_invariant, ((~Int.Le $__i2) $__n0)) (assume_measure_pos, ((~Int.Ge ((~Int.Sub $__n0) $__i2)) #0))
-(pre, ((~Int.Ge $__n0) #0))
+(<label_ite_cond_true: (~Int.Lt i n)>, (~Int.Lt #0 $__n0))
+(assume_guard, (~Int.Lt
+ $__i2
+ $__n0)) (assume_invariant, (~Int.Le $__i2 $__n0)) (assume_measure_pos, (~Int.Ge (~Int.Sub $__n0 $__i2) #0))
+(pre, (~Int.Ge $__n0 #0))
 
 Proof Obligation:
-((~Int.Lt ((~Int.Sub $__n0) ((~Int.Add $__i2) #1))) ((~Int.Sub $__n0) $__i2))
+(~Int.Lt (~Int.Sub $__n0 (~Int.Add $__i2 #1)) (~Int.Sub $__n0 $__i2))
 
 Label: measure_imp_not_guard
 Property: assert
 Assumptions:
-(<label_ite_cond_true: ((~Int.Lt i) n)>, ((~Int.Lt #0) $__n0))
-(assume_guard, ((~Int.Lt $__i2) $__n0)) (assume_invariant, ((~Int.Le $__i2) $__n0)) (assume_measure_pos, ((~Int.Ge ((~Int.Sub $__n0) $__i2)) #0))
-(pre, ((~Int.Ge $__n0) #0))
+(<label_ite_cond_true: (~Int.Lt i n)>, (~Int.Lt #0 $__n0))
+(assume_guard, (~Int.Lt
+ $__i2
+ $__n0)) (assume_invariant, (~Int.Le $__i2 $__n0)) (assume_measure_pos, (~Int.Ge (~Int.Sub $__n0 $__i2) #0))
+(pre, (~Int.Ge $__n0 #0))
 
 Proof Obligation:
-(if ((~Int.Le ((~Int.Sub $__n0) ((~Int.Add $__i2) #1))) #0) then (~Bool.Not ((~Int.Lt ((~Int.Add $__i2) #1)) $__n0)) else #true)
+(if (~Int.Le (~Int.Sub $__n0 (~Int.Add $__i2 #1)) #0) then (~Bool.Not (~Int.Lt (~Int.Add $__i2 #1) $__n0)) else #true)
 
 Label: arbitrary_iter_maintain_invariant
 Property: assert
 Assumptions:
-(<label_ite_cond_true: ((~Int.Lt i) n)>, ((~Int.Lt #0) $__n0))
-(assume_guard, ((~Int.Lt $__i2) $__n0)) (assume_invariant, ((~Int.Le $__i2) $__n0)) (assume_measure_pos, ((~Int.Ge ((~Int.Sub $__n0) $__i2)) #0))
-(pre, ((~Int.Ge $__n0) #0))
+(<label_ite_cond_true: (~Int.Lt i n)>, (~Int.Lt #0 $__n0))
+(assume_guard, (~Int.Lt
+ $__i2
+ $__n0)) (assume_invariant, (~Int.Le $__i2 $__n0)) (assume_measure_pos, (~Int.Ge (~Int.Sub $__n0 $__i2) #0))
+(pre, (~Int.Ge $__n0 #0))
 
 Proof Obligation:
-((~Int.Le ((~Int.Add $__i2) #1)) $__n0)
+(~Int.Le (~Int.Add $__i2 #1) $__n0)
 
 Label: i_eq_n
 Property: assert
 Assumptions:
-(pre, ((~Int.Ge $__n0) #0))
-(<label_ite_cond_true: ((~Int.Lt i) n)>, (if ((~Int.Lt #0) $__n0) then ((~Int.Lt #0) $__n0) else #true)) (assume_guard, (if ((~Int.Lt #0) $__n0) then ((~Int.Lt $__i2) $__n0) else #true)) (assume_invariant, (if ((~Int.Lt #0) $__n0) then ((~Int.Le $__i2) $__n0) else #true)) (assume_measure_pos, (if ((~Int.Lt #0) $__n0) then ((~Int.Ge ((~Int.Sub $__n0) $__i2)) #0) else #true)) (not_guard, (if ((~Int.Lt #0) $__n0) then (~Bool.Not ((~Int.Lt $__i3) $__n0)) else #true)) (invariant, (if ((~Int.Lt #0) $__n0) then ((~Int.Le $__i3) $__n0) else #true)) (<label_ite_cond_false: !((~Int.Lt i) n)>, (if (if ((~Int.Lt #0) $__n0) then #false else #true) then (if ((~Int.Lt #0) $__n0) then #false else #true) else #true))
+(pre, (~Int.Ge $__n0 #0))
+(<label_ite_cond_true: (~Int.Lt i n)>, (if (~Int.Lt
+  #0
+  $__n0) then (~Int.Lt
+  #0
+  $__n0) else #true)) (assume_guard, (if (~Int.Lt
+  #0
+  $__n0) then (~Int.Lt
+  $__i2
+  $__n0) else #true)) (assume_invariant, (if (~Int.Lt
+  #0
+  $__n0) then (~Int.Le
+  $__i2
+  $__n0) else #true)) (assume_measure_pos, (if (~Int.Lt
+  #0
+  $__n0) then (~Int.Ge
+  (~Int.Sub $__n0 $__i2)
+  #0) else #true)) (not_guard, (if (~Int.Lt
+  #0
+  $__n0) then (~Bool.Not
+  (~Int.Lt
+   $__i3
+   $__n0)) else #true)) (invariant, (if (~Int.Lt
+  #0
+  $__n0) then (~Int.Le
+  $__i3
+  $__n0) else #true)) (<label_ite_cond_false: !(~Int.Lt i n)>, (if (if (~Int.Lt
+   #0
+   $__n0) then #false else #true) then (if (~Int.Lt #0 $__n0) then #false else #true) else #true))
 
 Proof Obligation:
-((if ((~Int.Lt #0) $__n0) then $__i3 else #0) == $__n0)
+((if (~Int.Lt #0 $__n0) then $__i3 else #0) == $__n0)
 
 Label: post
 Property: assert
 Assumptions:
-(pre, ((~Int.Ge $__n0) #0))
-(<label_ite_cond_true: ((~Int.Lt i) n)>, (if ((~Int.Lt #0) $__n0) then ((~Int.Lt #0) $__n0) else #true)) (assume_guard, (if ((~Int.Lt #0) $__n0) then ((~Int.Lt $__i2) $__n0) else #true)) (assume_invariant, (if ((~Int.Lt #0) $__n0) then ((~Int.Le $__i2) $__n0) else #true)) (assume_measure_pos, (if ((~Int.Lt #0) $__n0) then ((~Int.Ge ((~Int.Sub $__n0) $__i2)) #0) else #true)) (not_guard, (if ((~Int.Lt #0) $__n0) then (~Bool.Not ((~Int.Lt $__i3) $__n0)) else #true)) (invariant, (if ((~Int.Lt #0) $__n0) then ((~Int.Le $__i3) $__n0) else #true)) (<label_ite_cond_false: !((~Int.Lt i) n)>, (if (if ((~Int.Lt #0) $__n0) then #false else #true) then (if ((~Int.Lt #0) $__n0) then #false else #true) else #true))
+(pre, (~Int.Ge $__n0 #0))
+(<label_ite_cond_true: (~Int.Lt i n)>, (if (~Int.Lt
+  #0
+  $__n0) then (~Int.Lt
+  #0
+  $__n0) else #true)) (assume_guard, (if (~Int.Lt
+  #0
+  $__n0) then (~Int.Lt
+  $__i2
+  $__n0) else #true)) (assume_invariant, (if (~Int.Lt
+  #0
+  $__n0) then (~Int.Le
+  $__i2
+  $__n0) else #true)) (assume_measure_pos, (if (~Int.Lt
+  #0
+  $__n0) then (~Int.Ge
+  (~Int.Sub $__n0 $__i2)
+  #0) else #true)) (not_guard, (if (~Int.Lt
+  #0
+  $__n0) then (~Bool.Not
+  (~Int.Lt
+   $__i3
+   $__n0)) else #true)) (invariant, (if (~Int.Lt
+  #0
+  $__n0) then (~Int.Le
+  $__i3
+  $__n0) else #true)) (<label_ite_cond_false: !(~Int.Lt i n)>, (if (if (~Int.Lt
+   #0
+   $__n0) then #false else #true) then (if (~Int.Lt #0 $__n0) then #false else #true) else #true))
 
 Proof Obligation:
 #true
