StrataTest/Languages/C_Simp/Examples/Min.lean
@@ -46,8 +46,14 @@ info: function min {
   pre: #true
   post: #true
   body:
-if ((~Int.Lt a) b) then {return := a}
-else{return := b}
+{
+  if (~Int.Lt a b) {
+    return := a
+  }
+  else {
+    return := b
+  }
+}
 }
 Errors: #[]
 -/
@@ -63,8 +69,10 @@ VCs:
 Label: post
 Property: assert
 Assumptions:
-(<label_ite_cond_true: ((~Int.Lt a) b)>, (if ((~Int.Lt $__a0) $__b1) then ((~Int.Lt $__a0) $__b1) else #true))
-(<label_ite_cond_false: !((~Int.Lt a) b)>, (if (if ((~Int.Lt $__a0) $__b1) then #false else #true) then (if ((~Int.Lt $__a0) $__b1) then #false else #true) else #true))
+(<label_ite_cond_true: (~Int.Lt a b)>, (if (~Int.Lt $__a0 $__b1) then (~Int.Lt $__a0 $__b1) else #true))
+(<label_ite_cond_false: !(~Int.Lt a b)>, (if (if (~Int.Lt
+   $__a0
+   $__b1) then #false else #true) then (if (~Int.Lt $__a0 $__b1) then #false else #true) else #true))
 
 Proof Obligation:
 #true
