StrataTest/Languages/Core/Examples/AdvancedQuantifiers.lean
@@ -33,17 +33,17 @@ Label: a
 Property: assert
 Assumptions:
 
-(mapAllValues0, (∀ (∀ (((~select %1) %0) == #0))))
+(mapAllValues0, (∀ (∀ ((~select %1 %0) == #0))))
 Proof Obligation:
-(((~select $__mArg0) $__kArg1) == #0)
+((~select $__mArg0 $__kArg1) == #0)
 
 Label: Update_ensures_0
 Property: assert
 Assumptions:
 
-(mapAllValues0, (∀ (∀ (((~select %1) %0) == #0))))
+(mapAllValues0, (∀ (∀ ((~select %1 %0) == #0))))
 Proof Obligation:
-(((~select $__mArg0) $__kArg1) == #0)
+((~select $__mArg0 $__kArg1) == #0)
 
 ---
 info:
