StrataTest/Languages/Core/Examples/DuplicateAssumeLabels.lean
@@ -40,20 +40,20 @@ VCs:
 Label: after_double_internal
 Property: assert
 Assumptions:
-(test, ((~Int.Ge $__n0) #2))
-(test_1, ((~Int.Ge $__n0) #0))
+(test, (~Int.Ge $__n0 #2))
+(test_1, (~Int.Ge $__n0 #0))
 
 Proof Obligation:
-((~Int.Ge ((~Int.Add $__n0) $__n0)) #4)
+(~Int.Ge (~Int.Add $__n0 $__n0) #4)
 
 Label: double_correct
 Property: assert
 Assumptions:
-(test, ((~Int.Ge $__n0) #2))
-(test_1, ((~Int.Ge $__n0) #0))
+(test, (~Int.Ge $__n0 #2))
+(test_1, (~Int.Ge $__n0 #0))
 
 Proof Obligation:
-(((~Int.Add $__n0) $__n0) == ((~Int.Mul $__n0) #2))
+((~Int.Add $__n0 $__n0) == (~Int.Mul $__n0 #2))
 
 ---
 info:
