StrataTest/Languages/Core/Examples/GeneratedLabels.lean
@@ -38,17 +38,51 @@ info: type Core.Boundedness.Infinite Ref []
 type Core.Boundedness.Infinite Field []
 type Struct := (Map Field int)
 type Heap := (Map Ref Struct)
-axiom axiom_0: (∀ (∀ (∀ (∀ (((~Bool.Implies : (arrow bool (arrow bool bool))) ((~Bool.Not : (arrow bool bool)) (%2 == %1))) ((((~select : (arrow (Map Field int) (arrow Field int))) %3) %2) == (((~select : (arrow (Map Field int) (arrow Field int))) ((((~update : (arrow (Map Field int) (arrow Field (arrow int (Map Field int))))) %3) %1) %0)) %2)))))));
-axiom axiom_1: (∀ (∀ (∀ ((((~select : (arrow (Map Field int) (arrow Field int))) ((((~update : (arrow (Map Field int) (arrow Field (arrow int (Map Field int))))) %2) %1) %0)) %1) == %0))));
-axiom axiom_2: (∀ (∀ (∀ (∀ (((~Bool.Implies : (arrow bool (arrow bool bool))) ((~Bool.Not : (arrow bool bool)) (%2 == %1))) ((((~select : (arrow (Map Ref Struct) (arrow Ref Struct))) %3) %2) == (((~select : (arrow (Map Ref Struct) (arrow Ref Struct))) ((((~update : (arrow (Map Ref Struct) (arrow Ref (arrow Struct (Map Ref Struct))))) %3) %1) %0)) %2)))))));
-axiom axiom_3: (∀ (∀ (∀ ((((~select : (arrow (Map Ref Struct) (arrow Ref Struct))) ((((~update : (arrow (Map Ref Struct) (arrow Ref (arrow Struct (Map Ref Struct))))) %2) %1) %0)) %1) == %0))));
+axiom axiom_0: (∀ (∀ (∀ (∀ ((~Bool.Implies : (arrow bool (arrow bool bool)))
+     ((~Bool.Not : (arrow bool bool)) (%2 == %1))
+     (((~select : (arrow (Map Field int) (arrow Field int)))
+       %3
+       %2) == ((~select : (arrow (Map Field int) (arrow Field int)))
+       ((~update : (arrow (Map Field int) (arrow Field (arrow int (Map Field int))))) %3 %1 %0)
+       %2)))))));
+axiom axiom_1: (∀ (∀ (∀ (((~select : (arrow (Map Field int) (arrow Field int)))
+     ((~update : (arrow (Map Field int) (arrow Field (arrow int (Map Field int))))) %2 %1 %0)
+     %1) == %0))));
+axiom axiom_2: (∀ (∀ (∀ (∀ ((~Bool.Implies : (arrow bool (arrow bool bool)))
+     ((~Bool.Not : (arrow bool bool)) (%2 == %1))
+     (((~select : (arrow (Map Ref Struct) (arrow Ref Struct)))
+       %3
+       %2) == ((~select : (arrow (Map Ref Struct) (arrow Ref Struct)))
+       ((~update : (arrow (Map Ref Struct) (arrow Ref (arrow Struct (Map Ref Struct))))) %3 %1 %0)
+       %2)))))));
+axiom axiom_3: (∀ (∀ (∀ (((~select : (arrow (Map Ref Struct) (arrow Ref Struct)))
+     ((~update : (arrow (Map Ref Struct) (arrow Ref (arrow Struct (Map Ref Struct))))) %2 %1 %0)
+     %1) == %0))));
 procedure test :  ((h : Heap) (ref : Ref) (field : Field)) → ()
   modifies: []
-  preconditions: ⏎
-  postconditions: ⏎
+  preconditions: 
+  postconditions: 
 {
-  init (newH : Heap) := ((((~update : (arrow (Map Ref Struct) (arrow Ref (arrow Struct (Map Ref Struct))))) (h : Heap)) (ref : Ref)) ((((~update : (arrow (Map Field int) (arrow Field (arrow int (Map Field int))))) (((~select : (arrow (Map Ref Struct) (arrow Ref Struct))) (h : Heap)) (ref : Ref))) (field : Field)) (((~Int.Add : (arrow int (arrow int int))) (((~select : (arrow (Map Field int) (arrow Field int))) (((~select : (arrow (Map Ref Struct) (arrow Ref Struct))) (h : Heap)) (ref : Ref))) (field : Field))) #1)))
-  assert [assert_0] ((((~select : (arrow (Map Field int) (arrow Field int))) (((~select : (arrow (Map Ref Struct) (arrow Ref Struct))) (newH : Heap)) (ref : Ref))) (field : Field)) == (((~Int.Add : (arrow int (arrow int int))) (((~select : (arrow (Map Field int) (arrow Field int))) (((~select : (arrow (Map Ref Struct) (arrow Ref Struct))) (h : Heap)) (ref : Ref))) (field : Field))) #1))
+  {
+    init (newH : Heap) := ((~update : (arrow (Map Ref Struct) (arrow Ref (arrow Struct (Map Ref Struct)))))
+     (h : Heap)
+     (ref : Ref)
+     ((~update : (arrow (Map Field int) (arrow Field (arrow int (Map Field int)))))
+      ((~select : (arrow (Map Ref Struct) (arrow Ref Struct))) (h : Heap) (ref : Ref))
+      (field : Field)
+      ((~Int.Add : (arrow int (arrow int int)))
+       ((~select : (arrow (Map Field int) (arrow Field int)))
+        ((~select : (arrow (Map Ref Struct) (arrow Ref Struct))) (h : Heap) (ref : Ref))
+        (field : Field))
+       #1)))
+    assert [assert_0] (((~select : (arrow (Map Field int) (arrow Field int)))
+      ((~select : (arrow (Map Ref Struct) (arrow Ref Struct))) (newH : Heap) (ref : Ref))
+      (field : Field)) == ((~Int.Add : (arrow int (arrow int int)))
+      ((~select : (arrow (Map Field int) (arrow Field int)))
+       ((~select : (arrow (Map Ref Struct) (arrow Ref Struct))) (h : Heap) (ref : Ref))
+       (field : Field))
+      #1))
+  }
 }
 -/
 #guard_msgs in
@@ -63,10 +97,23 @@ Label: assert_0
 Property: assert
 Assumptions:
 
-(axiom_0, (∀ (∀ (∀ (∀ ((~Bool.Implies (~Bool.Not (%2 == %1))) (((~select %3) %2) == ((~select (((~update %3) %1) %0)) %2))))))))
-(axiom_1, (∀ (∀ (∀ (((~select (((~update %2) %1) %0)) %1) == %0))))) (axiom_2, (∀ (∀ (∀ (∀ ((~Bool.Implies (~Bool.Not (%2 == %1))) (((~select %3) %2) == ((~select (((~update %3) %1) %0)) %2)))))))) (axiom_3, (∀ (∀ (∀ (((~select (((~update %2) %1) %0)) %1) == %0)))))
+(axiom_0, (∀ (∀ (∀ (∀ (~Bool.Implies (~Bool.Not (%2 == %1)) ((~select %3 %2) == (~select (~update %3 %1 %0) %2))))))))
+(axiom_1, (∀ (∀ (∀ ((~select
+     (~update %2 %1 %0)
+     %1) == %0))))) (axiom_2, (∀ (∀ (∀ (∀ (~Bool.Implies
+     (~Bool.Not (%2 == %1))
+     ((~select
+       %3
+       %2) == (~select (~update %3 %1 %0) %2)))))))) (axiom_3, (∀ (∀ (∀ ((~select (~update %2 %1 %0) %1) == %0)))))
 Proof Obligation:
-(((~select ((~select (((~update $__h0) $__ref1) (((~update ((~select $__h0) $__ref1)) $__field2) ((~Int.Add ((~select ((~select $__h0) $__ref1)) $__field2)) #1)))) $__ref1)) $__field2) == ((~Int.Add ((~select ((~select $__h0) $__ref1)) $__field2)) #1))
+((~select
+  (~select
+   (~update
+    $__h0
+    $__ref1
+    (~update (~select $__h0 $__ref1) $__field2 (~Int.Add (~select (~select $__h0 $__ref1) $__field2) #1)))
+   $__ref1)
+  $__field2) == (~Int.Add (~select (~select $__h0 $__ref1) $__field2) #1))
 
 ---
 info:
