StrataTest/Languages/Core/Examples/Regex.lean
@@ -58,7 +58,7 @@ Assumptions:
 
 
 Proof Obligation:
-(~Bool.Not ((~Str.InRegEx #hello.) ~cannot_end_with_period))
+(~Bool.Not (~Str.InRegEx #hello. ~cannot_end_with_period))
 
 Label: dot_ends_with_period
 Property: assert
@@ -66,7 +66,7 @@ Assumptions:
 
 
 Proof Obligation:
-(~Bool.Not ((~Str.InRegEx #.) ~cannot_end_with_period))
+(~Bool.Not (~Str.InRegEx #. ~cannot_end_with_period))
 
 Label: bye_exclaim_no_end_with_period
 Property: assert
@@ -74,7 +74,7 @@ Assumptions:
 
 
 Proof Obligation:
-((~Str.InRegEx #bye!) ~cannot_end_with_period)
+(~Str.InRegEx #bye! ~cannot_end_with_period)
 
 Label: ok_chars_str
 Property: assert
@@ -82,7 +82,7 @@ Assumptions:
 
 
 Proof Obligation:
-((~Str.InRegEx #test-str-1) ~ok_chars_regex)
+(~Str.InRegEx #test-str-1 ~ok_chars_regex)
 
 Label: cannot_contain_exclaim
 Property: assert
@@ -90,7 +90,7 @@ Assumptions:
 
 
 Proof Obligation:
-(~Bool.Not ((~Str.InRegEx #test-str!) ~ok_chars_regex))
+(~Bool.Not (~Str.InRegEx #test-str! ~ok_chars_regex))
 
 Label: has_to_be_at_least_1_char
 Property: assert
@@ -98,7 +98,7 @@ Assumptions:
 
 
 Proof Obligation:
-(~Bool.Not ((~Str.InRegEx #) ~ok_chars_regex))
+(~Bool.Not (~Str.InRegEx # ~ok_chars_regex))
 
 Label: cannot_exceed_10_chars
 Property: assert
@@ -106,7 +106,7 @@ Assumptions:
 
 
 Proof Obligation:
-(~Bool.Not ((~Str.InRegEx #0123456789a) ~ok_chars_regex))
+(~Bool.Not (~Str.InRegEx #0123456789a ~ok_chars_regex))
 
 Label: optionally_a_check1
 Property: assert
@@ -114,7 +114,7 @@ Assumptions:
 
 
 Proof Obligation:
-((~Str.InRegEx #a) ~optionally_a)
+(~Str.InRegEx #a ~optionally_a)
 
 Label: optionally_a_check2
 Property: assert
@@ -122,7 +122,7 @@ Assumptions:
 
 
 Proof Obligation:
-(~Bool.Not ((~Str.InRegEx #b) ~optionally_a))
+(~Bool.Not (~Str.InRegEx #b ~optionally_a))
 
 ---
 info:
@@ -201,7 +201,7 @@ Assumptions:
 
 
 Proof Obligation:
-(~Bool.Not ((~Str.InRegEx #0123456789a) (~bad_re_loop $__n0)))
+(~Bool.Not (~Str.InRegEx #0123456789a (~bad_re_loop $__n0)))
 
 Label: assert_1
 Property: assert
@@ -209,61 +209,71 @@ Assumptions:
 
 
 Proof Obligation:
-((~Str.InRegEx #a) (~bad_re_loop #1))
+(~Str.InRegEx #a (~bad_re_loop #1))
 
 
 
 Result: Obligation: assert_0
 Property: assert
 Result: 🚨 Implementation Error! SMT Encoding Error! Natural numbers expected as indices for re.loop.
-Original expression: (((~Re.Loop ((~Re.Range #a) #z)) #1) %0)
+Original expression: (~Re.Loop (~Re.Range #a #z) #1 %0)
 
 
 Evaluated program:
 func bad_re_loop :  ((n : int)) → regex :=
-  (((((~Re.Loop : (arrow regex (arrow int (arrow int regex)))) (((~Re.Range : (arrow string (arrow string regex))) #a) #z)) #1) (n : int)))
+  (((~Re.Loop : (arrow regex (arrow int (arrow int regex))))
+   ((~Re.Range : (arrow string (arrow string regex))) #a #z)
+   #1
+   (n : int)))
 procedure main :  ((n : int)) → ()
   modifies: []
-  preconditions: ⏎
-  postconditions: ⏎
+  preconditions: 
+  postconditions: 
 {
-  init (n1 : int) := init_n1_0
-  n1 := #1
-  assert [assert_0] (~Bool.Not ((~Str.InRegEx #0123456789a) (~bad_re_loop $__n0)))
-  assert [assert_1] ((~Str.InRegEx #a) (~bad_re_loop #1))
+  {
+    init (n1 : int) := init_n1_0
+    n1 := #1
+    assert [assert_0] (~Bool.Not (~Str.InRegEx #0123456789a (~bad_re_loop $__n0)))
+    assert [assert_1] (~Str.InRegEx #a (~bad_re_loop #1))
+  }
 }
 
 
 Result: Obligation: assert_1
 Property: assert
 Result: 🚨 Implementation Error! SMT Encoding Error! Natural numbers expected as indices for re.loop.
-Original expression: (((~Re.Loop ((~Re.Range #a) #z)) #1) %0)
+Original expression: (~Re.Loop (~Re.Range #a #z) #1 %0)
 
 
 Evaluated program:
 func bad_re_loop :  ((n : int)) → regex :=
-  (((((~Re.Loop : (arrow regex (arrow int (arrow int regex)))) (((~Re.Range : (arrow string (arrow string regex))) #a) #z)) #1) (n : int)))
+  (((~Re.Loop : (arrow regex (arrow int (arrow int regex))))
+   ((~Re.Range : (arrow string (arrow string regex))) #a #z)
+   #1
+   (n : int)))
 procedure main :  ((n : int)) → ()
   modifies: []
-  preconditions: ⏎
-  postconditions: ⏎
+  preconditions: 
+  postconditions: 
 {
-  init (n1 : int) := init_n1_0
-  n1 := #1
-  assert [assert_0] (~Bool.Not ((~Str.InRegEx #0123456789a) (~bad_re_loop $__n0)))
-  assert [assert_1] ((~Str.InRegEx #a) (~bad_re_loop #1))
+  {
+    init (n1 : int) := init_n1_0
+    n1 := #1
+    assert [assert_0] (~Bool.Not (~Str.InRegEx #0123456789a (~bad_re_loop $__n0)))
+    assert [assert_1] (~Str.InRegEx #a (~bad_re_loop #1))
+  }
 }
 ---
 info:
 Obligation: assert_0
 Property: assert
 Result: 🚨 Implementation Error! SMT Encoding Error! Natural numbers expected as indices for re.loop.
-Original expression: (((~Re.Loop ((~Re.Range #a) #z)) #1) %0)
+Original expression: (~Re.Loop (~Re.Range #a #z) #1 %0)
 
 Obligation: assert_1
 Property: assert
 Result: 🚨 Implementation Error! SMT Encoding Error! Natural numbers expected as indices for re.loop.
-Original expression: (((~Re.Loop ((~Re.Range #a) #z)) #1) %0)
+Original expression: (~Re.Loop (~Re.Range #a #z) #1 %0)
 -/
 #guard_msgs in
 #eval verify "cvc5" regexPgm2
@@ -293,7 +303,7 @@ Assumptions:
 
 
 Proof Obligation:
-(~Bool.Not ((~Str.InRegEx init_s_0) ~Re.None))
+(~Bool.Not (~Str.InRegEx init_s_0 ~Re.None))
 
 ---
 info:
