StrataTest/Languages/Core/Examples/SimpleProc.lean
@@ -35,10 +35,13 @@ spec {
 info: var (g : bool) := init_g_0
 procedure Test :  ((x : bool)) → ((y : bool))
   modifies: []
-  preconditions: ⏎
-  postconditions: (Test_ensures_0, ((y : bool) == (x : bool))) (Test_ensures_1, ((x : bool) == (y : bool))) (Test_ensures_2, ((g : bool) == ((~old : (arrow a a)) (g : bool))))
+  preconditions: 
+  postconditions: (Test_ensures_0, ((y : bool) == (x : bool))) (Test_ensures_1, ((x : bool) == (y : bool))) (Test_ensures_2, ((g : bool) == ((~old : (arrow a a))
+    (g : bool))))
 {
-  y := (((~Bool.Or : (arrow bool (arrow bool bool))) (x : bool)) (x : bool))
+  {
+    y := ((~Bool.Or : (arrow bool (arrow bool bool))) (x : bool) (x : bool))
+  }
 }
 Errors: #[]
 -/
@@ -56,7 +59,7 @@ Assumptions:
 
 
 Proof Obligation:
-(((~Bool.Or $__x0) $__x0) == $__x0)
+((~Bool.Or $__x0 $__x0) == $__x0)
 
 Label: Test_ensures_1
 Property: assert
@@ -64,7 +67,7 @@ Assumptions:
 
 
 Proof Obligation:
-($__x0 == ((~Bool.Or $__x0) $__x0))
+($__x0 == (~Bool.Or $__x0 $__x0))
 
 Label: Test_ensures_2
 Property: assert
