StrataTest/Languages/Core/Examples/TypeVarImplicitlyQuantified.lean
@@ -43,8 +43,14 @@ info: [Strata.Core] Type checking succeeded.
 info: ok: type set := (Map int bool)
 func diff :  ((a : (Map int bool)) (b : (Map int bool))) → (Map int bool);
 func lambda_0 :  ((l_0 : bool) (l_1 : int) (l_2 : int)) → (Map int int);
-axiom a1: (∀ (∀ ((((~diff : (arrow (Map int bool) (arrow (Map int bool) (Map int bool)))) %1) %0) == (((~diff : (arrow (Map int bool) (arrow (Map int bool) (Map int bool)))) %0) %1))));
-axiom a2: (∀ (∀ (∀ (∀ ((((~select : (arrow (Map int int) (arrow int int))) ((((~lambda_0 : (arrow bool (arrow int (arrow int (Map int int))))) %3) %2) %1)) %0) == (((~select : (arrow (Map int int) (arrow int int))) ((((~lambda_0 : (arrow bool (arrow int (arrow int (Map int int))))) %3) %1) %2)) %0))))));
+axiom a1: (∀ (∀ (((~diff : (arrow (Map int bool) (arrow (Map int bool) (Map int bool))))
+    %1
+    %0) == ((~diff : (arrow (Map int bool) (arrow (Map int bool) (Map int bool)))) %0 %1))));
+axiom a2: (∀ (∀ (∀ (∀ (((~select : (arrow (Map int int) (arrow int int)))
+      ((~lambda_0 : (arrow bool (arrow int (arrow int (Map int int))))) %3 %2 %1)
+      %0) == ((~select : (arrow (Map int int) (arrow int int)))
+      ((~lambda_0 : (arrow bool (arrow int (arrow int (Map int int))))) %3 %1 %2)
+      %0))))));
 -/
 #guard_msgs in
 #eval Core.typeCheck Options.default core_pgm.fst
