StrataTest/Languages/Core/ProcedureTypeTests.lean
@@ -17,13 +17,15 @@ open Procedure Statement Lambda Lambda.LTy.Syntax Lambda.LExpr.SyntaxMono Core.S
 /--
 info: ok: (procedure P :  ((x : int)) → ((y : int))
    modifies: []
-   preconditions: (0_lt_x, (((~Int.Lt : (arrow int (arrow int bool))) #0) (x : int)))
-   postconditions: (ret_y_lt_0, (((~Int.Lt : (arrow int (arrow int bool))) (y : int)) #0))
+   preconditions: (0_lt_x, ((~Int.Lt : (arrow int (arrow int bool))) #0 (x : int)))
+   postconditions: (ret_y_lt_0, ((~Int.Lt : (arrow int (arrow int bool))) (y : int) #0))
  {
-   y := (((~Int.Sub : (arrow int (arrow int int))) #0) (x : int))
+   {
+     y := ((~Int.Sub : (arrow int (arrow int int))) #0 (x : int))
+   }
  },
  context:
- types:   ⏎
+ types:   
  aliases: [] state: tyGen: 6 tyPrefix: $__ty exprGen: 0 exprPrefix: $__var subst: [])
 -/
 #guard_msgs in
@@ -46,10 +48,14 @@ info: ok: (procedure P :  ((x : int)) → ((y : int))
 /--
 info: ok: procedure P :  ((a : int)) → ()
   modifies: [g]
-  preconditions: ⏎
-  postconditions: (P.g_eq_a, ((g : int) == (((~Int.Add : (arrow int (arrow int int))) ((~old : (arrow int int)) (g : int))) (a : int))))
+  preconditions: 
+  postconditions: (P.g_eq_a, ((g : int) == ((~Int.Add : (arrow int (arrow int int)))
+    ((~old : (arrow int int)) (g : int))
+    (a : int))))
 {
-  g := (((~Int.Add : (arrow int (arrow int int))) (a : int)) (g : int))
+  {
+    g := ((~Int.Add : (arrow int (arrow int int))) (a : int) (g : int))
+  }
 }
 -/
 #guard_msgs in
@@ -76,10 +82,14 @@ info: ok: procedure P :  ((a : int)) → ()
 /--
 info: ok: procedure P :  ((a : int)) → ()
   modifies: [g]
-  preconditions: ⏎
-  postconditions: (P.g_eq_a, ((g : int) == (((~Int.Add : (arrow int (arrow int int))) ((~old : (arrow int int)) (a : int))) ((~old : (arrow int int)) (g : int)))))
+  preconditions: 
+  postconditions: (P.g_eq_a, ((g : int) == ((~Int.Add : (arrow int (arrow int int)))
+    ((~old : (arrow int int)) (a : int))
+    ((~old : (arrow int int)) (g : int)))))
 {
-  g := (((~Int.Add : (arrow int (arrow int int))) (a : int)) (g : int))
+  {
+    g := ((~Int.Add : (arrow int (arrow int int))) (a : int) (g : int))
+  }
 }
 -/
 #guard_msgs in
