StrataTest/Languages/Python/Regex/ReToCoreTests.lean
@@ -11,164 +11,229 @@ namespace Strata.Python.Tests
 open Strata.Python
 
 /--
-info: (((~Re.Concat ((~Re.Concat (~Str.ToRegEx #a)) (~Str.ToRegEx #b))) ((~Re.Union ((~Re.Union (~Str.ToRegEx #)) ~Re.AllChar)) ((~Re.Concat ((~Re.Concat ~Re.AllChar) (~Re.Star ~Re.AllChar))) ~Re.AllChar))),
+info: ((~Re.Concat
+  (~Re.Concat (~Str.ToRegEx #a) (~Str.ToRegEx #b))
+  (~Re.Union
+   (~Re.Union (~Str.ToRegEx #) ~Re.AllChar)
+   (~Re.Concat (~Re.Concat ~Re.AllChar (~Re.Star ~Re.AllChar)) ~Re.AllChar))),
  none)
 -/
 #guard_msgs in
 #eval Std.format$ pythonRegexToCore "ab.*" -- Encoded as `ab(|.|..*.)`
 
 /--
-info: (((~Re.Concat ((~Re.Concat (~Str.ToRegEx #a)) (~Str.ToRegEx #b))) ((~Re.Union ((~Re.Union (~Str.ToRegEx #)) ((~Re.Concat (~Str.ToRegEx #c)) (~Str.ToRegEx #)))) ((~Re.Concat ((~Re.Concat ((~Re.Concat (~Str.ToRegEx #c)) ~Re.None)) (~Re.Star ((~Re.Concat (~Str.ToRegEx #c)) ~Re.None)))) ((~Re.Concat (~Str.ToRegEx #c)) (~Str.ToRegEx #))))),
+info: ((~Re.Concat
+  (~Re.Concat (~Str.ToRegEx #a) (~Str.ToRegEx #b))
+  (~Re.Union
+   (~Re.Union (~Str.ToRegEx #) (~Re.Concat (~Str.ToRegEx #c) (~Str.ToRegEx #)))
+   (~Re.Concat
+    (~Re.Concat (~Re.Concat (~Str.ToRegEx #c) ~Re.None) (~Re.Star (~Re.Concat (~Str.ToRegEx #c) ~Re.None)))
+    (~Re.Concat (~Str.ToRegEx #c) (~Str.ToRegEx #))))),
  none)
 -/
 #guard_msgs in
 #eval Std.format$ pythonRegexToCore "ab(c$)*"
 
 /--
-info: (((~Re.Concat ((~Re.Concat (~Str.ToRegEx #a)) (~Str.ToRegEx #b))) ((~Re.Union ((~Re.Union (~Str.ToRegEx #)) ((~Re.Concat ((~Re.Concat ~Re.None) (~Str.ToRegEx #c))) (~Str.ToRegEx #)))) ((~Re.Concat ((~Re.Concat ((~Re.Concat ((~Re.Concat ~Re.None) (~Str.ToRegEx #c))) ~Re.None)) (~Re.Star ((~Re.Concat ((~Re.Concat ~Re.None) (~Str.ToRegEx #c))) ~Re.None)))) ((~Re.Concat ((~Re.Concat ~Re.None) (~Str.ToRegEx #c))) (~Str.ToRegEx #))))),
+info: ((~Re.Concat
+  (~Re.Concat (~Str.ToRegEx #a) (~Str.ToRegEx #b))
+  (~Re.Union
+   (~Re.Union (~Str.ToRegEx #) (~Re.Concat (~Re.Concat ~Re.None (~Str.ToRegEx #c)) (~Str.ToRegEx #)))
+   (~Re.Concat
+    (~Re.Concat
+     (~Re.Concat (~Re.Concat ~Re.None (~Str.ToRegEx #c)) ~Re.None)
+     (~Re.Star (~Re.Concat (~Re.Concat ~Re.None (~Str.ToRegEx #c)) ~Re.None)))
+    (~Re.Concat (~Re.Concat ~Re.None (~Str.ToRegEx #c)) (~Str.ToRegEx #))))),
  none)
 -/
 #guard_msgs in
 #eval Std.format$ pythonRegexToCore "ab(^c$)*"
 
-/-- info: (((~Re.Concat (~Str.ToRegEx #a)) (~Str.ToRegEx #b)), none) -/
+/--
+info: ((~Re.Concat (~Str.ToRegEx #a) (~Str.ToRegEx #b)), none)
+-/
 #guard_msgs in
 #eval Std.format$ pythonRegexToCore "ab"
 
-/-- info: (((~Re.Union (~Str.ToRegEx #a)) (~Str.ToRegEx #b)), none) -/
+/--
+info: ((~Re.Union (~Str.ToRegEx #a) (~Str.ToRegEx #b)), none)
+-/
 #guard_msgs in
 #eval Std.format$ pythonRegexToCore "a|b"
 
 /--
-info: (((~Re.Concat ((~Re.Concat (~Str.ToRegEx #)) (~Str.ToRegEx #a))) (~Str.ToRegEx #b)), none)
+info: ((~Re.Concat (~Re.Concat (~Str.ToRegEx #) (~Str.ToRegEx #a)) (~Str.ToRegEx #b)), none)
 -/
 #guard_msgs in
 #eval Std.format$ pythonRegexToCore "^ab"
 
 /--
-info: (((~Re.Concat ((~Re.Concat ((~Re.Concat (~Str.ToRegEx #)) (~Str.ToRegEx #a))) (~Str.ToRegEx #b))) (~Str.ToRegEx #)),
- none)
+info: ((~Re.Concat (~Re.Concat (~Re.Concat (~Str.ToRegEx #) (~Str.ToRegEx #a)) (~Str.ToRegEx #b)) (~Str.ToRegEx #)), none)
 -/
 #guard_msgs in
 #eval Std.format$ pythonRegexToCore "^ab$"
 
-/-- info: (((~Re.Concat ((~Re.Concat (~Str.ToRegEx #a)) ~Re.None)) (~Str.ToRegEx #b)), none) -/
+/--
+info: ((~Re.Concat (~Re.Concat (~Str.ToRegEx #a) ~Re.None) (~Str.ToRegEx #b)), none)
+-/
 #guard_msgs in
 #eval Std.format$ pythonRegexToCore "(a$)b"
 
 /--
-info: (((~Re.Concat ((~Re.Concat ((~Re.Concat ((~Re.Concat ((~Re.Concat (~Str.ToRegEx #)) (~Str.ToRegEx #))) (~Str.ToRegEx #))) (~Str.ToRegEx #a))) (~Str.ToRegEx #))) (~Str.ToRegEx #)),
+info: ((~Re.Concat
+  (~Re.Concat
+   (~Re.Concat (~Re.Concat (~Re.Concat (~Str.ToRegEx #) (~Str.ToRegEx #)) (~Str.ToRegEx #)) (~Str.ToRegEx #a))
+   (~Str.ToRegEx #))
+  (~Str.ToRegEx #)),
  none)
 -/
 #guard_msgs in
 #eval Std.format $ pythonRegexToCore "^^^a$$"
 
 /--
-info: (((~Re.Concat (~Str.ToRegEx #)) ((~Re.Concat ((~Re.Concat ((~Re.Concat ((~Re.Concat (~Str.ToRegEx #)) (~Str.ToRegEx #))) (~Str.ToRegEx #a))) (~Str.ToRegEx #))) (~Str.ToRegEx #))),
+info: ((~Re.Concat
+  (~Str.ToRegEx #)
+  (~Re.Concat
+   (~Re.Concat (~Re.Concat (~Re.Concat (~Str.ToRegEx #) (~Str.ToRegEx #)) (~Str.ToRegEx #a)) (~Str.ToRegEx #))
+   (~Str.ToRegEx #))),
  none)
 -/
 #guard_msgs in
 #eval Std.format $ pythonRegexToCore "^(^^a$$)"
 
 /--
-info: (((~Re.Union ((~Re.Concat ((~Re.Concat (~Str.ToRegEx #)) (~Str.ToRegEx #a))) (~Str.ToRegEx #))) ((~Re.Concat ((~Re.Concat (~Str.ToRegEx #)) (~Str.ToRegEx #b))) (~Str.ToRegEx #))),
+info: ((~Re.Union
+  (~Re.Concat (~Re.Concat (~Str.ToRegEx #) (~Str.ToRegEx #a)) (~Str.ToRegEx #))
+  (~Re.Concat (~Re.Concat (~Str.ToRegEx #) (~Str.ToRegEx #b)) (~Str.ToRegEx #))),
  none)
 -/
 #guard_msgs in
 #eval Std.format $ pythonRegexToCore "(^a$)|(^b$)"
 
 /--
-info: (((~Re.Concat (~Str.ToRegEx #c)) ((~Re.Union ((~Re.Concat ~Re.None) (~Str.ToRegEx #a))) ((~Re.Concat ~Re.None) (~Str.ToRegEx #b)))),
+info: ((~Re.Concat
+  (~Str.ToRegEx #c)
+  (~Re.Union (~Re.Concat ~Re.None (~Str.ToRegEx #a)) (~Re.Concat ~Re.None (~Str.ToRegEx #b)))),
  none)
 -/
 #guard_msgs in
 #eval Std.format $ pythonRegexToCore "c((^a)|(^b))"
 
 /--
-info: (((~Re.Concat ((~Re.Union ((~Re.Concat (~Str.ToRegEx #a)) ~Re.None)) ((~Re.Concat (~Str.ToRegEx #b)) ~Re.None))) (~Str.ToRegEx #c)),
+info: ((~Re.Concat
+  (~Re.Union (~Re.Concat (~Str.ToRegEx #a) ~Re.None) (~Re.Concat (~Str.ToRegEx #b) ~Re.None))
+  (~Str.ToRegEx #c)),
  none)
 -/
 #guard_msgs in
 #eval Std.format $ pythonRegexToCore "((a$)|(b$))c"
 
 /--
-info: (((~Re.Concat ((~Re.Union ((~Re.Concat (~Str.ToRegEx #a)) ~Re.None)) (~Str.ToRegEx #b))) (~Str.ToRegEx #c)), none)
+info: ((~Re.Concat (~Re.Union (~Re.Concat (~Str.ToRegEx #a) ~Re.None) (~Str.ToRegEx #b)) (~Str.ToRegEx #c)), none)
 -/
 #guard_msgs in
 #eval Std.format $ pythonRegexToCore "((a$)|(b))c"
 
 /--
-info: (((~Re.Concat (~Str.ToRegEx #c)) ((~Re.Union ((~Re.Concat (~Str.ToRegEx #a)) (~Str.ToRegEx #))) ((~Re.Concat ((~Re.Concat ~Re.None) (~Str.ToRegEx #b))) (~Str.ToRegEx #)))),
+info: ((~Re.Concat
+  (~Str.ToRegEx #c)
+  (~Re.Union
+   (~Re.Concat (~Str.ToRegEx #a) (~Str.ToRegEx #))
+   (~Re.Concat (~Re.Concat ~Re.None (~Str.ToRegEx #b)) (~Str.ToRegEx #)))),
  none)
 -/
 #guard_msgs in
 #eval Std.format $ pythonRegexToCore "c((a$)|(^b$))"
 
 /--
-info: (((~Re.Concat ((~Re.Union ((~Re.Concat (~Str.ToRegEx #a)) ~Re.None)) (~Str.ToRegEx #b))) (~Str.ToRegEx #c)), none)
+info: ((~Re.Concat (~Re.Union (~Re.Concat (~Str.ToRegEx #a) ~Re.None) (~Str.ToRegEx #b)) (~Str.ToRegEx #c)), none)
 -/
 #guard_msgs in
 #eval Std.format $ pythonRegexToCore "((a$)|(b))c"
 
-/-- info: (((~Re.Concat ((~Re.Concat (~Str.ToRegEx #)) ~Re.None)) (~Str.ToRegEx #b)), none) -/
+/--
+info: ((~Re.Concat (~Re.Concat (~Str.ToRegEx #) ~Re.None) (~Str.ToRegEx #b)), none)
+-/
 #guard_msgs in
 #eval Std.format $ pythonRegexToCore "^$b"
 
 /--
-info: (((~Re.Union ((~Re.Concat ((~Re.Concat (~Str.ToRegEx #)) (~Str.ToRegEx #a))) (~Str.ToRegEx #))) ((~Re.Concat ((~Re.Concat (~Str.ToRegEx #)) ~Re.None)) (~Str.ToRegEx #b))),
+info: ((~Re.Union
+  (~Re.Concat (~Re.Concat (~Str.ToRegEx #) (~Str.ToRegEx #a)) (~Str.ToRegEx #))
+  (~Re.Concat (~Re.Concat (~Str.ToRegEx #) ~Re.None) (~Str.ToRegEx #b))),
  none)
 -/
 #guard_msgs in
 #eval Std.format $ pythonRegexToCore "^a$|^$b"
 
 /--
-info: (((~Re.Concat ((~Re.Concat (~Str.ToRegEx #c)) ((~Re.Union ((~Re.Concat ~Re.None) (~Str.ToRegEx #a))) ((~Re.Concat (~Str.ToRegEx #b)) ~Re.None)))) (~Str.ToRegEx #d)),
+info: ((~Re.Concat
+  (~Re.Concat
+   (~Str.ToRegEx #c)
+   (~Re.Union (~Re.Concat ~Re.None (~Str.ToRegEx #a)) (~Re.Concat (~Str.ToRegEx #b) ~Re.None)))
+  (~Str.ToRegEx #d)),
  none)
 -/
 #guard_msgs in
 #eval Std.format $ pythonRegexToCore "c(^a|b$)d"
 
 /--
-info: (((~Re.Concat ((~Re.Concat (~Str.ToRegEx #c)) ((~Re.Union ((~Re.Concat ~Re.None) (~Str.ToRegEx #a))) ((~Re.Concat (~Str.ToRegEx #b)) ~Re.None)))) (~Str.ToRegEx #d)),
+info: ((~Re.Concat
+  (~Re.Concat
+   (~Str.ToRegEx #c)
+   (~Re.Union (~Re.Concat ~Re.None (~Str.ToRegEx #a)) (~Re.Concat (~Str.ToRegEx #b) ~Re.None)))
+  (~Str.ToRegEx #d)),
  none)
 -/
 #guard_msgs in
 #eval Std.format $ pythonRegexToCore "(c(^a|b$))d"
 
 /--
-info: (((~Re.Concat ((~Re.Union ((~Re.Concat (~Str.ToRegEx #)) (~Str.ToRegEx #a))) ((~Re.Concat (~Str.ToRegEx #b)) ~Re.None))) ((~Re.Union ((~Re.Concat ~Re.None) (~Str.ToRegEx #c))) ((~Re.Concat (~Str.ToRegEx #d)) (~Str.ToRegEx #)))),
+info: ((~Re.Concat
+  (~Re.Union (~Re.Concat (~Str.ToRegEx #) (~Str.ToRegEx #a)) (~Re.Concat (~Str.ToRegEx #b) ~Re.None))
+  (~Re.Union (~Re.Concat ~Re.None (~Str.ToRegEx #c)) (~Re.Concat (~Str.ToRegEx #d) (~Str.ToRegEx #)))),
  none)
 -/
 #guard_msgs in
 #eval Std.format $ pythonRegexToCore "(^a|b$)(^c|d$)"
 
 /--
-info: (((~Re.Concat ((~Re.Concat ((~Re.Union ((~Re.Concat (~Str.ToRegEx #)) (~Str.ToRegEx #a))) ((~Re.Concat (~Str.ToRegEx #b)) ~Re.None))) ~Re.None)) (~Str.ToRegEx #c)),
+info: ((~Re.Concat
+  (~Re.Concat
+   (~Re.Union (~Re.Concat (~Str.ToRegEx #) (~Str.ToRegEx #a)) (~Re.Concat (~Str.ToRegEx #b) ~Re.None))
+   ~Re.None)
+  (~Str.ToRegEx #c)),
  none)
 -/
 #guard_msgs in
 #eval Std.format $ pythonRegexToCore "((^a|b$)^)c"
 
-/-- info: (((~Re.Concat ((~Re.Union (~Str.ToRegEx #)) ~Re.None)) (~Str.ToRegEx #c)), none) -/
+/--
+info: ((~Re.Concat (~Re.Union (~Str.ToRegEx #) ~Re.None) (~Str.ToRegEx #c)), none)
+-/
 #guard_msgs in
 #eval Std.format $ pythonRegexToCore "(^|$)c"
 
-/-- info: (((~Re.Concat (~Str.ToRegEx #)) (~Str.ToRegEx #)), none) -/
+/--
+info: ((~Re.Concat (~Str.ToRegEx #) (~Str.ToRegEx #)), none)
+-/
 #guard_msgs in
 #eval Std.format $ pythonRegexToCore "^^"
 
 /--
-info: (((~Re.Concat ((~Re.Concat ((~Re.Concat (~Str.ToRegEx #)) (~Str.ToRegEx #))) (~Str.ToRegEx #))) (~Str.ToRegEx #)), none)
+info: ((~Re.Concat (~Re.Concat (~Re.Concat (~Str.ToRegEx #) (~Str.ToRegEx #)) (~Str.ToRegEx #)) (~Str.ToRegEx #)), none)
 -/
 #guard_msgs in
 #eval Std.format $ pythonRegexToCore "^$$^"
 
-/-- info: (((~Re.Concat ((~Re.Union (~Str.ToRegEx #)) (~Str.ToRegEx #))) (~Str.ToRegEx #)), none) -/
+/--
+info: ((~Re.Concat (~Re.Union (~Str.ToRegEx #) (~Str.ToRegEx #)) (~Str.ToRegEx #)), none)
+-/
 #guard_msgs in
 #eval Std.format $ pythonRegexToCore "(^|$)^"
 
 /--
-info: (((~Re.Concat ((~Re.Concat (~Str.ToRegEx #)) (~Str.ToRegEx #a))) (~Str.ToRegEx #)), none)
+info: ((~Re.Concat (~Re.Concat (~Str.ToRegEx #) (~Str.ToRegEx #a)) (~Str.ToRegEx #)), none)
 -/
 #guard_msgs in
 #eval Std.format $ pythonRegexToCore "^a$" .fullmatch
@@ -181,17 +246,21 @@ info: (~Re.All,
 #eval Std.format $ pythonRegexToCore "x{100,2}" .fullmatch
 
 -- (unmatchable)
-/-- info: (((~Re.Concat ((~Re.Concat (~Str.ToRegEx #a)) ~Re.None)) (~Str.ToRegEx #b)), none) -/
+/--
+info: ((~Re.Concat (~Re.Concat (~Str.ToRegEx #a) ~Re.None) (~Str.ToRegEx #b)), none)
+-/
 #guard_msgs in
 #eval Std.format $ pythonRegexToCore "a^b" .fullmatch
 
 /--
-info: (((~Re.Concat ((~Re.Concat ((~Re.Concat (~Str.ToRegEx #)) (~Str.ToRegEx #a))) ~Re.None)) (~Str.ToRegEx #b)), none)
+info: ((~Re.Concat (~Re.Concat (~Re.Concat (~Str.ToRegEx #) (~Str.ToRegEx #a)) ~Re.None) (~Str.ToRegEx #b)), none)
 -/
 #guard_msgs in
 #eval Std.format $ pythonRegexToCore "^a^b" .fullmatch
 
-/-- info: (((~Re.Concat ((~Re.Concat (~Str.ToRegEx #a)) ~Re.None)) (~Str.ToRegEx #b)), none) -/
+/--
+info: ((~Re.Concat (~Re.Concat (~Str.ToRegEx #a) ~Re.None) (~Str.ToRegEx #b)), none)
+-/
 #guard_msgs in
 #eval Std.format $ pythonRegexToCore "a$b" .fullmatch
 
@@ -199,7 +268,9 @@ info: (((~Re.Concat ((~Re.Concat ((~Re.Concat (~Str.ToRegEx #)) (~Str.ToRegEx #a
 #guard_msgs in
 #eval Std.format $ pythonRegexToCore "[^b]" .fullmatch
 
-/-- info: ((~Re.Comp ((~Re.Range #A) #Z)), none) -/
+/--
+info: ((~Re.Comp (~Re.Range #A #Z)), none)
+-/
 #guard_msgs in
 #eval Std.format $ pythonRegexToCore "[^A-Z]" .fullmatch
 
@@ -212,7 +283,11 @@ info: (((~Re.Concat ((~Re.Concat ((~Re.Concat (~Str.ToRegEx #)) (~Str.ToRegEx #a
 #eval Std.format $ pythonRegexToCore "a" .fullmatch
 
 /--
-info: (((~Re.Concat (~Str.ToRegEx #a)) ((~Re.Union ((~Re.Union (~Str.ToRegEx #)) ~Re.AllChar)) ((~Re.Concat ((~Re.Concat ~Re.AllChar) (~Re.Star ~Re.AllChar))) ~Re.AllChar))),
+info: ((~Re.Concat
+  (~Str.ToRegEx #a)
+  (~Re.Union
+   (~Re.Union (~Str.ToRegEx #) ~Re.AllChar)
+   (~Re.Concat (~Re.Concat ~Re.AllChar (~Re.Star ~Re.AllChar)) ~Re.AllChar))),
  none)
 -/
 #guard_msgs in
@@ -220,20 +295,38 @@ info: (((~Re.Concat (~Str.ToRegEx #a)) ((~Re.Union ((~Re.Union (~Str.ToRegEx #))
 
 -- search mode tests
 /--
-info: (((~Re.Concat ((~Re.Union ((~Re.Union (~Str.ToRegEx #)) ~Re.AllChar)) ((~Re.Concat ((~Re.Concat ~Re.AllChar) (~Re.Star ~Re.AllChar))) ~Re.AllChar))) ((~Re.Concat (~Str.ToRegEx #a)) ((~Re.Union ((~Re.Union (~Str.ToRegEx #)) ~Re.AllChar)) ((~Re.Concat ((~Re.Concat ~Re.AllChar) (~Re.Star ~Re.AllChar))) ~Re.AllChar)))),
+info: ((~Re.Concat
+  (~Re.Union
+   (~Re.Union (~Str.ToRegEx #) ~Re.AllChar)
+   (~Re.Concat (~Re.Concat ~Re.AllChar (~Re.Star ~Re.AllChar)) ~Re.AllChar))
+  (~Re.Concat
+   (~Str.ToRegEx #a)
+   (~Re.Union
+    (~Re.Union (~Str.ToRegEx #) ~Re.AllChar)
+    (~Re.Concat (~Re.Concat ~Re.AllChar (~Re.Star ~Re.AllChar)) ~Re.AllChar)))),
  none)
 -/
 #guard_msgs in
 #eval Std.format $ pythonRegexToCore "a" .search
 
 /--
-info: (((~Re.Concat ((~Re.Union ((~Re.Union (~Str.ToRegEx #)) ~Re.AllChar)) ((~Re.Concat ((~Re.Concat ~Re.AllChar) (~Re.Star ~Re.AllChar))) ~Re.AllChar))) ((~Re.Concat ((~Re.Concat ((~Re.Concat (~Str.ToRegEx #)) (~Str.ToRegEx #a))) (~Str.ToRegEx #))) ((~Re.Union ((~Re.Union (~Str.ToRegEx #)) ~Re.AllChar)) ((~Re.Concat ((~Re.Concat ~Re.AllChar) (~Re.Star ~Re.AllChar))) ~Re.AllChar)))),
+info: ((~Re.Concat
+  (~Re.Union
+   (~Re.Union (~Str.ToRegEx #) ~Re.AllChar)
+   (~Re.Concat (~Re.Concat ~Re.AllChar (~Re.Star ~Re.AllChar)) ~Re.AllChar))
+  (~Re.Concat
+   (~Re.Concat (~Re.Concat (~Str.ToRegEx #) (~Str.ToRegEx #a)) (~Str.ToRegEx #))
+   (~Re.Union
+    (~Re.Union (~Str.ToRegEx #) ~Re.AllChar)
+    (~Re.Concat (~Re.Concat ~Re.AllChar (~Re.Star ~Re.AllChar)) ~Re.AllChar)))),
  none)
 -/
 #guard_msgs in
 #eval Std.format $ pythonRegexToCore "^a$" .search
 
-/-- info: (((~Re.Concat (~Str.ToRegEx #)) (~Str.ToRegEx #a)), none) -/
+/--
+info: ((~Re.Concat (~Str.ToRegEx #) (~Str.ToRegEx #a)), none)
+-/
 #guard_msgs in
 #eval Std.format $ pythonRegexToCore "^a" .fullmatch
 
